Proof sketches for [strictly precedes]

src/Operational.thy
@@ -61,6 +61,9 @@ inductive operational_semantics_elim :: "('\<tau>::linordered_field) config \<Ri
 | precedes_e:
   "(\<Gamma>, n \<turnstile> ((K\<^sub>1 precedes K\<^sub>2) # \<Psi>) \<triangleright> \<Phi>)
      \<hookrightarrow>\<^sub>e  (((\<lceil>#\<^sup>\<le> K\<^sub>2 n, #\<^sup>< K\<^sub>1 n\<rceil> \<in> (\<lambda>(x,y). x\<le>y)) # \<Gamma>), n \<turnstile> \<Psi> \<triangleright> ((K\<^sub>1 precedes K\<^sub>2) # \<Phi>))"
+| strictly_precedes_e:
+  "(\<Gamma>, n \<turnstile> ((K\<^sub>1 strictly precedes K\<^sub>2) # \<Psi>) \<triangleright> \<Phi>)
+     \<hookrightarrow>\<^sub>e  (((\<lceil>#\<^sup>\<le> K\<^sub>2 n, #\<^sup>< K\<^sub>1 n\<rceil> \<in> (\<lambda>(x,y). x<y)) # \<Gamma>), n \<turnstile> \<Psi> \<triangleright> ((K\<^sub>1 strictly precedes K\<^sub>2) # \<Phi>))"
 
 inductive operational_semantics_step :: "('\<tau>::linordered_field) config \<Rightarrow> '\<tau> config \<Rightarrow> bool" ("_ \<hookrightarrow> _" 70) where
     intro_part: "(\<Gamma>\<^sub>1, n\<^sub>1 \<turnstile> \<Psi>\<^sub>1 \<triangleright> \<Phi>\<^sub>1)  \<hookrightarrow>\<^sub>i  (\<Gamma>\<^sub>2, n\<^sub>2 \<turnstile> \<Psi>\<^sub>2 \<triangleright> \<Phi>\<^sub>2)
@@ -146,6 +149,11 @@ lemma Cnext_solve_precedes:
   shows "(\<C>\<^sub>n\<^sub>e\<^sub>x\<^sub>t (\<Gamma>, n \<turnstile> ((K\<^sub>1 precedes K\<^sub>2) # \<Psi>) \<triangleright> \<Phi>))
           \<supseteq> { ((\<lceil>#\<^sup>\<le> K\<^sub>2 n, #\<^sup>< K\<^sub>1 n\<rceil> \<in> (\<lambda>(x,y). x\<le>y)) # \<Gamma>), n \<turnstile> \<Psi> \<triangleright> ((K\<^sub>1 precedes K\<^sub>2) # \<Phi>) }"
   by (simp add: operational_semantics_step.simps operational_semantics_elim.precedes_e)
+
+lemma Cnext_solve_strictly_precedes:
+  shows "(\<C>\<^sub>n\<^sub>e\<^sub>x\<^sub>t (\<Gamma>, n \<turnstile> ((K\<^sub>1 strictly precedes K\<^sub>2) # \<Psi>) \<triangleright> \<Phi>))
+          \<supseteq> { ((\<lceil>#\<^sup>\<le> K\<^sub>2 n, #\<^sup>< K\<^sub>1 n\<rceil> \<in> (\<lambda>(x,y). x<y)) # \<Gamma>), n \<turnstile> \<Psi> \<triangleright> ((K\<^sub>1 strictly precedes K\<^sub>2) # \<Phi>) }"
+  by (simp add: operational_semantics_step.simps operational_semantics_elim.strictly_precedes_e)
 
 lemma empty_spec_reductions:
   shows "([], 0 \<turnstile> [] \<triangleright> []) \<hookrightarrow>\<^bsup>k\<^esup> ([], k \<turnstile> [] \<triangleright> [])"
