src/Coinductive_Prop.thy
@@ -32,6 +32,8 @@ fun TESL_interpretation_atomic_stepwise
         }"
   | "\<lbrakk> K\<^sub>1 precedes K\<^sub>2 \<rbrakk>\<^sub>T\<^sub>E\<^sub>S\<^sub>L\<^bsup>\<ge> i\<^esup> =
         { \<rho>. \<forall>n\<ge>i. (run_tick_count \<rho> K\<^sub>2 n) \<le> (run_tick_count_strictly \<rho> K\<^sub>1 n) }"
+  | "\<lbrakk> K\<^sub>1 strictly precedes K\<^sub>2 \<rbrakk>\<^sub>T\<^sub>E\<^sub>S\<^sub>L\<^bsup>\<ge> i\<^esup> =
+        { \<rho>. \<forall>n\<ge>i. (run_tick_count \<rho> K\<^sub>2 n) < (run_tick_count_strictly \<rho> K\<^sub>1 n) }"
 
 theorem predicate_Inter_unfold:
   "{ \<rho>. \<forall>n. P \<rho> n} = \<Inter> {Y. \<exists>n. Y = { \<rho>. P \<rho> n }}"
@@ -76,6 +78,10 @@ lemma TESL_interp_unfold_stepwise_precedes:
   shows "\<lbrakk> K\<^sub>1 precedes K\<^sub>2 \<rbrakk>\<^sub>T\<^sub>E\<^sub>S\<^sub>L = \<Inter> {Y. \<exists>n::nat. Y = \<lbrakk> K\<^sub>1 precedes K\<^sub>2 \<rbrakk>\<^sub>T\<^sub>E\<^sub>S\<^sub>L\<^bsup>\<ge> n\<^esup>}"
   by auto
 
+lemma TESL_interp_unfold_stepwise_strictly_precedes:
+  shows "\<lbrakk> K\<^sub>1 strictly precedes K\<^sub>2 \<rbrakk>\<^sub>T\<^sub>E\<^sub>S\<^sub>L = \<Inter> {Y. \<exists>n::nat. Y = \<lbrakk> K\<^sub>1 strictly precedes K\<^sub>2 \<rbrakk>\<^sub>T\<^sub>E\<^sub>S\<^sub>L\<^bsup>\<ge> n\<^esup>}"
+  by auto
+
 theorem TESL_interp_unfold_stepwise_positive_atoms:
   assumes "positive_atom \<phi>"
   shows "\<lbrakk> \<phi>::'\<tau>::linordered_field TESL_atomic \<rbrakk>\<^sub>T\<^sub>E\<^sub>S\<^sub>L = \<Union> {Y. \<exists>n::nat. Y = \<lbrakk> \<phi> \<rbrakk>\<^sub>T\<^sub>E\<^sub>S\<^sub>L\<^bsup>\<ge> n\<^esup>}"
@@ -115,6 +121,10 @@ next
   case (Precedes x61 x62)
   then show ?thesis
     using TESL_interp_unfold_stepwise_precedes by simp
+next
+  case (StrictlyPrecedes x61 x62)
+  then show ?thesis
+    using TESL_interp_unfold_stepwise_strictly_precedes by simp
 qed
 
 lemma forall_nat_expansion:
@@ -282,6 +292,12 @@ lemma TESL_interp_stepwise_precedes_coind_unfold:
     then show ?thesis by auto
   qed
 
+lemma TESL_interp_stepwise_strictly_precedes_coind_unfold:
+  shows "\<lbrakk> K\<^sub>1 strictly precedes K\<^sub>2 \<rbrakk>\<^sub>T\<^sub>E\<^sub>S\<^sub>L\<^bsup>\<ge> n\<^esup> =
+    \<lbrakk> (\<lceil>#\<^sup>\<le> K\<^sub>2 n, #\<^sup>< K\<^sub>1 n\<rceil> \<in> (\<lambda>(x,y). x<y)) \<rbrakk>\<^sub>p\<^sub>r\<^sub>i\<^sub>m
+    \<inter> \<lbrakk> K\<^sub>1 strictly precedes K\<^sub>2 \<rbrakk>\<^sub>T\<^sub>E\<^sub>S\<^sub>L\<^bsup>\<ge> Suc n\<^esup>"
+  sorry
+
 fun TESL_interpretation_stepwise :: "'\<tau>::linordered_field TESL_formula \<Rightarrow> nat \<Rightarrow> '\<tau> run set" ("\<lbrakk>\<lbrakk> _ \<rbrakk>\<rbrakk>\<^sub>T\<^sub>E\<^sub>S\<^sub>L\<^bsup>\<ge> _\<^esup>") where
     "\<lbrakk>\<lbrakk> [] \<rbrakk>\<rbrakk>\<^sub>T\<^sub>E\<^sub>S\<^sub>L\<^bsup>\<ge> n\<^esup> = { _. True }"
   | "\<lbrakk>\<lbrakk> \<phi> # \<Phi> \<rbrakk>\<rbrakk>\<^sub>T\<^sub>E\<^sub>S\<^sub>L\<^bsup>\<ge> n\<^esup> = \<lbrakk> \<phi> \<rbrakk>\<^sub>T\<^sub>E\<^sub>S\<^sub>L\<^bsup>\<ge> n\<^esup> \<inter> \<lbrakk>\<lbrakk> \<Phi> \<rbrakk>\<rbrakk>\<^sub>T\<^sub>E\<^sub>S\<^sub>L\<^bsup>\<ge> n\<^esup>"
@@ -335,6 +351,9 @@ lemma TESL_interpretation_stepwise_zero:
     then show ?case by simp
   next
     case (Precedes x1 x2)
+    then show ?case by simp
+  next
+    case (StrictlyPrecedes x1 x2)
     then show ?case by simp
   qed
 
@@ -548,5 +567,10 @@ lemma HeronConf_interp_stepwise_precedes_cases':
   shows "\<lbrakk> \<Gamma>, n \<turnstile> ((K\<^sub>1 precedes K\<^sub>2) # \<Psi>) \<triangleright> \<Phi> \<rbrakk>\<^sub>c\<^sub>o\<^sub>n\<^sub>f\<^sub>i\<^sub>g
           = \<lbrakk> ((#\<^sup>\<le> K\<^sub>2 n \<preceq> #\<^sup>< K\<^sub>1 n) # \<Gamma>), n \<turnstile> \<Psi> \<triangleright> ((K\<^sub>1 precedes K\<^sub>2) # \<Phi>) \<rbrakk>\<^sub>c\<^sub>o\<^sub>n\<^sub>f\<^sub>i\<^sub>g"
   oops
+
+lemma HeronConf_interp_stepwise_strictly_precedes_cases:
+  shows "\<lbrakk> \<Gamma>, n \<turnstile> ((K\<^sub>1 strictly precedes K\<^sub>2) # \<Psi>) \<triangleright> \<Phi> \<rbrakk>\<^sub>c\<^sub>o\<^sub>n\<^sub>f\<^sub>i\<^sub>g
+          = \<lbrakk> ((\<lceil>#\<^sup>\<le> K\<^sub>2 n, #\<^sup>< K\<^sub>1 n\<rceil> \<in> (\<lambda>(x,y). x<y)) # \<Gamma>), n \<turnstile> \<Psi> \<triangleright> ((K\<^sub>1 strictly precedes K\<^sub>2) # \<Phi>) \<rbrakk>\<^sub>c\<^sub>o\<^sub>n\<^sub>f\<^sub>i\<^sub>g"
+  sorry
 
 end
