src/Denotational.thy
@@ -15,8 +15,6 @@ fun TESL_interpretation_atomic
   | "\<lbrakk> K\<^sub>1 sporadic \<lparr>\<tau>\<^sub>v\<^sub>a\<^sub>r(K\<^sub>i, n\<^sub>i) \<oplus> \<delta>\<tau>\<rparr> on K\<^sub>2 \<rbrakk>\<^sub>T\<^sub>E\<^sub>S\<^sub>L =
         { \<rho>. \<exists>n::nat. hamlet ((Rep_run \<rho>) n K\<^sub>1) = True
                        \<and> time ((Rep_run \<rho>) n K\<^sub>2) = time ((Rep_run \<rho>) n\<^sub>i K\<^sub>i) + \<delta>\<tau> }"
-  (* | "\<lbrakk> tag-relation K\<^sub>1 = \<alpha> * K\<^sub>2 + \<beta> \<rbrakk>\<^sub>T\<^sub>E\<^sub>S\<^sub>L =
-        { \<rho>. \<forall>n::nat. time ((Rep_run \<rho>) n K\<^sub>1) = \<alpha> * time ((Rep_run \<rho>) n K\<^sub>2) + \<beta> }" *)
   | "\<lbrakk> tag-relation \<lfloor>K\<^sub>1, K\<^sub>2\<rfloor> \<in> R \<rbrakk>\<^sub>T\<^sub>E\<^sub>S\<^sub>L =
         { \<rho>. \<forall>n::nat. R (time ((Rep_run \<rho>) n K\<^sub>1), time ((Rep_run \<rho>) n K\<^sub>2)) }"
   | "\<lbrakk> master implies slave \<rbrakk>\<^sub>T\<^sub>E\<^sub>S\<^sub>L =
@@ -32,6 +30,8 @@ fun TESL_interpretation_atomic
         }"
   | "\<lbrakk> K\<^sub>1 precedes K\<^sub>2 \<rbrakk>\<^sub>T\<^sub>E\<^sub>S\<^sub>L =
         { \<rho>. \<forall>n::nat. (run_tick_count \<rho> K\<^sub>2 n) \<le> (run_tick_count_strictly \<rho> K\<^sub>1 n) }"
+  | "\<lbrakk> K\<^sub>1 strictly precedes K\<^sub>2 \<rbrakk>\<^sub>T\<^sub>E\<^sub>S\<^sub>L =
+        { \<rho>. \<forall>n::nat. (run_tick_count \<rho> K\<^sub>2 n) < (run_tick_count_strictly \<rho> K\<^sub>1 n) }"
 
 section \<open>Denotational interpretation for TESL formulae\<close>
 
